immutable-btree/BtreeBenchmark.dfy
@@ -3,21 +3,21 @@ include "BtreeSpec.dfy"
 include "BtreeInv.dfy"  
 //include "BtreeImpl.dfy"
 
-module Integer_BtreeSpec refines BtreeSpec {
-  import Keyspace = Bounded_Integer_Order
-}
-
-module Integer_BtreeInv refines BtreeInv {
-  import opened Spec = Integer_BtreeSpec
-}
-
 method Main() {
+    var tree = BtreeImpl.empty();
+
     var nInsertions := 1000 * 1000 * 10;
     var i := 0;
     while i < nInsertions
+    invariant WFTree(tree)
     {
         var v := (i * 1073741827) % nInsertions;
+        var w := (i * 1234141827) % nInsertions;
         i := i + 1;
+
+        var k = Bounded_Integer_Order.Element(v);
+
+        tree = BtreeImpl.put(tree, k, w);
     }
 }
 
